matching-logic/src/Theories/DeductionTheorem.v
@@ -1,0 +1,1459 @@
+(*
+  This file contains admits for some cases of well formedness.
+  Those cases are indeed well formed and could be reasoned about by hand.
+  However, time is better spent by making wf_auto2 be able to fix them.
+*)
+
+From Coq Require Import ssreflect ssrfun ssrbool.
+
+From Ltac2 Require Import Ltac2.
+
+Require Import Equations.Prop.Equations.
+
+From Coq Require Import String Ensembles Setoid.
+Require Import Coq.Program.Equality.
+Require Import Coq.Logic.Classical_Prop.
+From Coq.Logic Require Import FunctionalExtensionality Eqdep_dec.
+From Coq.Classes Require Import Morphisms_Prop.
+From Coq.Unicode Require Import Utf8.
+From Coq.micromega Require Import Lia.
+
+From stdpp Require Import base fin_sets sets propset proof_irrel option list coGset finite infinite gmap.
+
+From MatchingLogic Require Import Logic
+                                  DerivedOperators_Syntax
+                                  ProofMode.
+From MatchingLogic.Theories Require Import Definedness_Syntax Definedness_ProofSystem.
+From MatchingLogic.Utils Require Import stdpp_ext.
+Import extralibrary.
+
+Import MatchingLogic.Logic.Notations.
+Import MatchingLogic.DerivedOperators_Syntax.Notations.
+Import MatchingLogic.Syntax.BoundVarSugar.
+
+Set Default Proof Mode "Classic".
+
+Import Notations.
+
+Open Scope ml_scope.
+Open Scope string_scope.
+Open Scope list_scope.
+
+(* TODO: These 3 lemmas are used only here as is, but maybe it should be somewhere else? *)
+Local Lemma impl_ctx_impl {Σ : Signature} Γ ctx ϕ ψ i :
+  well_formed ϕ ->
+  well_formed ψ ->
+  well_formed (pcPattern ctx) ->
+  ProofInfoLe AnyReasoning i ->
+  Γ ⊢i ϕ ---> ψ using i ->
+  (is_positive_context ctx ->
+  Γ ⊢i (emplace ctx ϕ) ---> (emplace ctx ψ) using i)
+  *
+  (is_negative_context ctx ->
+  Γ ⊢i (emplace ctx ψ) ---> (emplace ctx ϕ) using i).
+Proof.
+  intros wfϕ wfψ wfc pile H.
+
+  remember (size' (pcPattern ctx)) as sz.
+  assert (Hsz: size' (pcPattern ctx) <= sz) by lia.
+  clear Heqsz.
+
+  unfold emplace.
+
+  destruct ctx as [cvar cpatt].
+  simpl in *.
+
+  generalize dependent cpatt.
+
+  induction sz.
+  {
+    destruct cpatt; simpl in *; lia.
+  }
+
+  intros cpatt wfc Hsz.
+
+  split.
+  {
+    intro Hp.
+    destruct cpatt; simpl in *.
+
+    (* trivial cases *)
+    2,5,7: aapply A_impl_A;[eapply pile_trans;[|apply pile];try_solve_pile;try_solve_pile|wf_auto2].
+    (* not well formed cases*)
+    2,3: cbv in wfc; discriminate wfc.
+
+    + destruct decide.
+      { assumption. }
+      { gapply A_impl_A. eapply pile_trans;[|apply pile]; try_solve_pile. wf_auto2. }
+
+    + pose proof (IH1 := IHsz cpatt1).
+      feed specialize IH1.
+      { wf_auto2. }
+      { lia. }
+      destruct IH1 as [IH1 _]. feed specialize IH1.
+      {
+        clear -Hp. unfold is_positive_context in *. simpl in *.
+        unfold evar_has_negative_occurrence in Hp.
+        simpl in Hp. fold evar_has_negative_occurrence in Hp.
+        rewrite negb_or in Hp. destruct_and! Hp.
+        assumption.
+      }
+      pose proof (IH2 := IHsz cpatt2).
+      feed specialize IH2.
+      { wf_auto2. }
+      { lia. }
+      destruct IH2 as [IH2 _]. feed specialize IH2.
+      {
+        clear -Hp. unfold is_positive_context in *. simpl in *.
+        unfold evar_has_negative_occurrence in Hp.
+        simpl in Hp. fold evar_has_negative_occurrence in Hp.
+        rewrite negb_or in Hp. destruct_and! Hp.
+        assumption.
+      }
+
+      eapply syllogism_meta.
+      4: {
+        unshelve(eapply Framing_left;[|apply IH1]).
+        { wf_auto2. }
+        { eapply pile_trans;[|apply pile]. apply pile_any. }
+      }
+      { wf_auto2. }
+      { wf_auto2. }
+      { wf_auto2. }
+      
+      unshelve(eapply Framing_right).
+      { wf_auto2. }
+      { eapply pile_trans;[|apply pile]. apply pile_any. }
+      apply IH2.
+
+    + unfold is_positive_context in Hp. simpl in Hp.
+      unfold evar_has_negative_occurrence in Hp. simpl in Hp.
+      fold evar_has_positive_occurrence evar_has_negative_occurrence in Hp.
+      rewrite negb_orb in Hp.
+      destruct_and! Hp.
+
+      pose proof (IH := IHsz (cpatt2)).
+      feed specialize IH.
+      { wf_auto2. }
+      { lia. }
+      destruct IH as [IH _]. feed specialize IH.
+      {
+        unfold is_positive_context. simpl. assumption.
+      }
+
+      toMLGoal.
+      { wf_auto2. }
+      mlAdd IH as "IH". clear IH.
+      mlIntro "H".
+      mlIntro "Hc".
+      mlApply "IH". mlClear "IH".
+      mlApply "H". mlClear "H".
+      fromMLGoal.
+
+      pose proof (IH := IHsz cpatt1).
+      feed specialize IH.
+      { wf_auto2. }
+      { lia. }
+      destruct IH as [_ IH]. feed specialize IH.
+      { unfold is_negative_context. simpl. assumption. }
+      assumption.
+
+    + remember (evar_fresh_s ({[cvar]} ∪ free_evars cpatt ∪ free_evars ψ ∪ free_evars ϕ)) as x.
+      pose proof (IH := IHsz (evar_open x 0 cpatt)).
+      feed specialize IH.
+      { wf_auto2. }
+      { rewrite evar_open_size'. lia. }
+      destruct IH as [IH _]. feed specialize IH.
+      {
+        clear -Hp Heqx. unfold is_positive_context in *. simpl in *.
+        unfold evar_has_negative_occurrence in Hp.
+        simpl in Hp. fold evar_has_negative_occurrence in Hp.
+        rewrite <- neg_occurrence_bevar_subst.
+        + assumption.
+        + subst. solve_fresh_neq.
+      }
+      rewrite <- evar_quantify_evar_open with (n := 0) (phi := cpatt^[[evar:cvar↦ϕ]]) (x := x).
+      rewrite <- evar_quantify_evar_open with (n := 0) (phi := cpatt^[[evar:cvar↦ψ]]) (x := x).
+      apply ex_quan_monotone.
+      { eapply pile_trans;[|apply pile]. try_solve_pile. }
+      unfold evar_open.
+      unfold evar_open in IH.
+
+      rewrite free_evar_subst_free_evar_subst.
+      { wf_auto2. }
+      {
+        apply count_evar_occurrences_0.
+        subst; clear; simpl.
+        rewrite not_elem_of_singleton.
+        solve_fresh_neq.
+      }
+
+      rewrite free_evar_subst_free_evar_subst.
+      { wf_auto2. }
+      {
+        apply count_evar_occurrences_0.
+        subst; clear; simpl.
+        rewrite not_elem_of_singleton.
+        solve_fresh_neq.
+      }
+
+      assumption.
+
+      {
+        subst x; clear.
+        eapply evar_is_fresh_in_richer'.
+        2: { apply set_evar_fresh_is_fresh'. }
+        pose proof (Hfree := free_evars_free_evar_subst cpatt ψ cvar).
+        set_solver.
+      }
+      { wf_auto2. }
+      {
+        subst x. 
+        eapply evar_is_fresh_in_richer'.
+        2: { apply set_evar_fresh_is_fresh'. }
+        pose proof (Hfree := free_evars_free_evar_subst cpatt ϕ cvar).
+        clear -Hfree.
+        set_solver.
+      }
+      { wf_auto2. }
+
+    + remember (svar_fresh_s (free_svars cpatt ∪ free_svars ψ ∪ free_svars ϕ ∪ free_svars cpatt^[[evar:cvar↦ϕ]] ∪ free_svars cpatt^[[evar:cvar↦ψ]])) as X.
+      pose proof (IH := IHsz (svar_open X 0 cpatt)).
+      feed specialize IH.
+      { wf_auto2. }
+      { rewrite svar_open_size'. lia. }
+      destruct IH as [IH _]. feed specialize IH.
+      {
+        clear -Hp. unfold is_positive_context in *. simpl in *.
+        cbn in Hp.
+        rewrite <- neg_occurrence_bsvar_subst.
+        assumption.
+      }
+      rewrite <- svar_quantify_svar_open with (n := 0) (phi := cpatt^[[evar:cvar↦ϕ]]) (X := X).
+      rewrite <- svar_quantify_svar_open with (n := 0) (phi := cpatt^[[evar:cvar↦ψ]]) (X := X).
+      apply mu_monotone.
+      { eapply pile_trans;[|apply pile]. try_solve_pile. }
+      {
+        unfold is_positive_context in Hp. simpl in Hp. 
+        unfold well_formed in wfc. simpl in wfc.
+        destruct_and! wfc.
+        pose proof (Hneg := free_evar_subst_preserves_no_negative_occurrence cvar cpatt ϕ 0).
+        feed specialize Hneg.
+        { wf_auto2. }
+        { assumption. }
+        cbn in Hp.
+        apply positive_negative_occurrence_db_named.
+        { assumption. }
+        apply fresh_svar_no_neg.
+        subst.
+        clear.
+        eapply svar_is_fresh_in_richer'.
+        2: apply set_svar_fresh_is_fresh'.
+        set_solver.
+      }
+      {
+        unfold is_positive_context in Hp. simpl in Hp. 
+        unfold well_formed in wfc. simpl in wfc.
+        destruct_and! wfc.
+        pose proof (Hneg := free_evar_subst_preserves_no_negative_occurrence cvar cpatt ψ 0).
+        feed specialize Hneg.
+        { wf_auto2. }
+        { assumption. }
+        cbn in Hp.
+        apply positive_negative_occurrence_db_named.
+        { assumption. }
+        apply fresh_svar_no_neg.
+        subst.
+        clear.
+        eapply svar_is_fresh_in_richer'.
+        2: apply set_svar_fresh_is_fresh'.
+        set_solver.
+      }
+      unfold svar_open.
+      unfold svar_open in IH.
+      rewrite <- free_evar_subst_bsvar_subst.
+      rewrite <- free_evar_subst_bsvar_subst.
+      apply IH.
+      { wf_auto2. }
+      { unfold evar_is_fresh_in. set_solver. }
+      { wf_auto2. }
+      { unfold evar_is_fresh_in. set_solver. }
+      {
+        clear -HeqX.
+        intro Hcontra.
+        pose proof (Hfree := free_svars_free_evar_subst cpatt cvar ψ).
+        assert (X ∉ free_svars cpatt /\ X ∉ free_svars ψ).
+        {
+          subst.
+          split.
+          {
+            eapply svar_is_fresh_in_richer'.
+            2: apply set_svar_fresh_is_fresh'.
+            clear.
+            set_solver.
+          }
+          {
+            eapply svar_is_fresh_in_richer'.
+            2: apply set_svar_fresh_is_fresh'.
+            clear.
+            set_solver.
+          }
+        }
+        set_solver.
+      }
+      { wf_auto2. }
+      {
+        subst X.
+        eapply svar_is_fresh_in_richer'.
+        2: apply set_svar_fresh_is_fresh'.
+        clear.
+        set_solver.
+      }
+      { wf_auto2. }
+  }
+  {
+    intro Hp.
+    destruct cpatt; simpl in *.
+
+    (* trivial cases *)
+    2,5,7: aapply A_impl_A;[eapply pile_trans;[|apply pile];try_solve_pile;try_solve_pile|wf_auto2].
+    (* not well formed cases*)
+    2,3: cbv in wfc; discriminate wfc.
+
+    + destruct decide.
+      {
+        subst.
+        unfold is_negative_context in Hp. cbn in Hp.
+        destruct decide in Hp; simpl in Hp; congruence.
+      }
+      { gapply A_impl_A. eapply pile_trans;[|apply pile]; try_solve_pile. wf_auto2. }
+
+    + pose proof (IH1 := IHsz cpatt1).
+      feed specialize IH1.
+      { wf_auto2. }
+      { lia. }
+      destruct IH1 as [_ IH1]. feed specialize IH1.
+      {
+        clear -Hp. unfold is_negative_context in *. simpl in *.
+        cbn in Hp.
+        rewrite negb_or in Hp. destruct_and! Hp.
+        assumption.
+      }
+      pose proof (IH2 := IHsz cpatt2).
+      feed specialize IH2.
+      { wf_auto2. }
+      { lia. }
+      destruct IH2 as [_ IH2]. feed specialize IH2.
+      {
+        clear -Hp. unfold is_negative_context in *. simpl in *.
+        cbn in Hp.
+        rewrite negb_or in Hp. destruct_and! Hp.
+        assumption.
+      }
+
+      eapply syllogism_meta.
+      4: {
+        unshelve(eapply Framing_left;[|apply IH1]).
+        { wf_auto2. }
+        { eapply pile_trans;[|apply pile]. apply pile_any. }
+      }
+      { wf_auto2. }
+      { wf_auto2. }
+      { wf_auto2. }
+      
+      unshelve(eapply Framing_right).
+      { wf_auto2. }
+      { eapply pile_trans;[|apply pile]. apply pile_any. }
+      apply IH2.
+
+    + unfold is_negative_context in Hp. simpl in Hp.
+      unfold evar_has_positive_occurrence in Hp. simpl in Hp.
+      fold evar_has_positive_occurrence evar_has_negative_occurrence in Hp.
+      rewrite negb_orb in Hp.
+      destruct_and! Hp.
+
+      pose proof (IH := IHsz (cpatt2)).
+      feed specialize IH.
+      { wf_auto2. }
+      { lia. }
+      destruct IH as [_ IH]. feed specialize IH.
+      {
+        unfold is_negative_context. simpl. assumption.
+      }
+
+      toMLGoal.
+      { wf_auto2. }
+      mlAdd IH as "IH". clear IH.
+      mlIntro "H".
+      mlIntro "Hc".
+      mlApply "IH". mlClear "IH".
+      mlApply "H". mlClear "H".
+      fromMLGoal.
+
+      pose proof (IH := IHsz cpatt1).
+      feed specialize IH.
+      { wf_auto2. }
+      { lia. }
+      destruct IH as [IH _]. feed specialize IH.
+      { unfold is_positive_context. simpl. assumption. }
+      assumption.
+
+    + remember (evar_fresh_s ({[cvar]} ∪ free_evars cpatt ∪ free_evars ψ ∪ free_evars ϕ)) as x.
+      pose proof (IH := IHsz (evar_open x 0 cpatt)).
+      feed specialize IH.
+      { wf_auto2. }
+      { rewrite evar_open_size'. lia. }
+      destruct IH as [_ IH]. feed specialize IH.
+      {
+        clear -Hp Heqx. unfold is_negative_context in *. simpl in *.
+        cbn in Hp.
+        rewrite <- pos_occurrence_bevar_subst.
+        + assumption.
+        + subst. solve_fresh_neq.
+      }
+      rewrite <- evar_quantify_evar_open with (n := 0) (phi := cpatt^[[evar:cvar↦ϕ]]) (x := x).
+      rewrite <- evar_quantify_evar_open with (n := 0) (phi := cpatt^[[evar:cvar↦ψ]]) (x := x).
+      apply ex_quan_monotone.
+      { eapply pile_trans;[|apply pile]. try_solve_pile. }
+      unfold evar_open.
+      unfold evar_open in IH.
+
+      rewrite free_evar_subst_free_evar_subst.
+      { wf_auto2. }
+      {
+        apply count_evar_occurrences_0.
+        subst; clear; simpl.
+        rewrite not_elem_of_singleton.
+        solve_fresh_neq.
+      }
+
+      rewrite free_evar_subst_free_evar_subst.
+      { wf_auto2. }
+      {
+        apply count_evar_occurrences_0.
+        subst; clear; simpl.
+        rewrite not_elem_of_singleton.
+        solve_fresh_neq.
+      }
+
+      assumption.
+
+      {
+        subst x; clear.
+        eapply evar_is_fresh_in_richer'.
+        2: { apply set_evar_fresh_is_fresh'. }
+        pose proof (Hfree := free_evars_free_evar_subst cpatt ψ cvar).
+        set_solver.
+      }
+      { wf_auto2. }
+      {
+        subst x. 
+        eapply evar_is_fresh_in_richer'.
+        2: { apply set_evar_fresh_is_fresh'. }
+        pose proof (Hfree := free_evars_free_evar_subst cpatt ϕ cvar).
+        clear -Hfree.
+        set_solver.
+      }
+      { wf_auto2. }
+
+    + remember (svar_fresh_s (free_svars cpatt ∪ free_svars ψ ∪ free_svars ϕ ∪ free_svars cpatt^[[evar:cvar↦ϕ]] ∪ free_svars cpatt^[[evar:cvar↦ψ]])) as X.
+      pose proof (IH := IHsz (svar_open X 0 cpatt)).
+      feed specialize IH.
+      { wf_auto2. }
+      { rewrite svar_open_size'. lia. }
+      destruct IH as [_ IH]. feed specialize IH.
+      {
+        clear -Hp. unfold is_negative_context in *. simpl in *.
+        cbn in Hp.
+        rewrite <- pos_occurrence_bsvar_subst.
+        assumption.
+      }
+      rewrite <- svar_quantify_svar_open with (n := 0) (phi := cpatt^[[evar:cvar↦ϕ]]) (X := X).
+      rewrite <- svar_quantify_svar_open with (n := 0) (phi := cpatt^[[evar:cvar↦ψ]]) (X := X).
+      apply mu_monotone.
+      { eapply pile_trans;[|apply pile]. try_solve_pile. }
+      {
+        unfold is_negative_context in Hp. simpl in Hp. 
+        unfold well_formed in wfc. simpl in wfc.
+        destruct_and! wfc.
+        pose proof (Hneg := free_evar_subst_preserves_no_negative_occurrence cvar cpatt ψ 0).
+        feed specialize Hneg.
+        { wf_auto2. }
+        { assumption. }
+        cbn in Hp.
+        apply positive_negative_occurrence_db_named.
+        { assumption. }
+        apply fresh_svar_no_neg.
+        subst.
+        clear.
+        eapply svar_is_fresh_in_richer'.
+        2: apply set_svar_fresh_is_fresh'.
+        set_solver.
+      }
+      {
+        unfold is_negative_context in Hp. simpl in Hp. 
+        unfold well_formed in wfc. simpl in wfc.
+        destruct_and! wfc.
+        pose proof (Hneg := free_evar_subst_preserves_no_negative_occurrence cvar cpatt ϕ 0).
+        feed specialize Hneg.
+        { wf_auto2. }
+        { assumption. }
+        cbn in Hp.
+        apply positive_negative_occurrence_db_named.
+        { assumption. }
+        apply fresh_svar_no_neg.
+        subst.
+        clear.
+        eapply svar_is_fresh_in_richer'.
+        2: apply set_svar_fresh_is_fresh'.
+        set_solver.
+      }
+      unfold svar_open.
+      unfold svar_open in IH.
+      rewrite <- free_evar_subst_bsvar_subst.
+      rewrite <- free_evar_subst_bsvar_subst.
+      apply IH.
+      { wf_auto2. }
+      { unfold evar_is_fresh_in. set_solver. }
+      { wf_auto2. }
+      { unfold evar_is_fresh_in. set_solver. }
+      {
+        clear -HeqX.
+        intro Hcontra.
+        pose proof (Hfree := free_svars_free_evar_subst cpatt cvar ψ).
+        assert (X ∉ free_svars cpatt /\ X ∉ free_svars ψ).
+        {
+          subst.
+          split.
+          {
+            eapply svar_is_fresh_in_richer'.
+            2: apply set_svar_fresh_is_fresh'.
+            clear.
+            set_solver.
+          }
+          {
+            eapply svar_is_fresh_in_richer'.
+            2: apply set_svar_fresh_is_fresh'.
+            clear.
+            set_solver.
+          }
+        }
+        set_solver.
+      }
+      { wf_auto2. }
+      {
+        subst X.
+        eapply svar_is_fresh_in_richer'.
+        2: apply set_svar_fresh_is_fresh'.
+        clear.
+        set_solver.
+      }
+      { wf_auto2. }
+  }
+Defined.
+
+Lemma impl_ctx_impl_pos {Σ : Signature} Γ ctx ϕ ψ i :
+  well_formed ϕ ->
+  well_formed ψ ->
+  well_formed (pcPattern ctx) ->
+  is_positive_context ctx ->
+  ProofInfoLe AnyReasoning i ->
+  Γ ⊢i ϕ ---> ψ using i ->
+  Γ ⊢i (emplace ctx ϕ) ---> (emplace ctx ψ) using i.
+Proof.
+  intros wfϕ wfψ wfc Hp pile H.
+  pose proof (impl := impl_ctx_impl Γ ctx ϕ ψ i wfϕ wfψ wfc pile H).
+  destruct impl as [impl _].
+  apply impl in Hp.
+  assumption.
+Defined.
+
+Lemma impl_ctx_impl_neg {Σ : Signature} Γ ctx ϕ ψ i :
+  well_formed ϕ ->
+  well_formed ψ ->
+  well_formed (pcPattern ctx) ->
+  is_negative_context ctx ->
+  ProofInfoLe AnyReasoning i ->
+  Γ ⊢i ϕ ---> ψ using i ->
+  Γ ⊢i (emplace ctx ψ) ---> (emplace ctx ϕ) using i.
+Proof.
+  intros wfϕ wfψ wfc Hn pile H.
+  pose proof (impl := impl_ctx_impl Γ ctx ϕ ψ i wfϕ wfψ wfc pile H).
+  destruct impl as [_ impl].
+  apply impl in Hn.
+  assumption.
+Defined.
+
+(* TODO:
+  This lemma is lemma 88 in in the matching mu logic paper.
+  As is there is no way to determine the mu requirement and
+  propagation of predicates is unproved.
+*)
+Lemma pred_and_ctx_and {Σ : Signature} {syntax : Syntax} Γ ctx ϕ ψ i :
+  well_formed ϕ ->
+  well_formed ψ ->
+  well_formed (pcPattern ctx) ->
+  Γ ⊢i is_predicate_pattern ψ using i ->
+  Γ ⊢i ψ and (emplace ctx ϕ) <---> ψ and (emplace ctx (ψ and ϕ)) using (ExGen := ∅, SVSubst := ∅, KT := false, FP := ∅).
+Proof.
+  intros wfm wfψ wfc Hp.
+
+  remember (size' (pcPattern ctx)) as sz.
+  assert (Hsz: size' (pcPattern ctx) <= sz) by lia.
+  clear Heqsz.
+
+  unfold emplace.
+
+  destruct ctx as [cvar cpatt].
+  simpl in *.
+
+  generalize dependent cpatt.
+
+  induction sz.
+  {
+    destruct cpatt; simpl in *; lia.
+  }
+
+  intros cpatt wfc Hsz.
+  destruct cpatt. all: simpl in *.
+
+  (* trivial cases *)
+  2,5,7: apply pf_iff_split;[wf_auto2|wf_auto2|aapply A_impl_A;[try_solve_pile|wf_auto2]|aapply A_impl_A;[try_solve_pile|wf_auto2] ].
+  (* not well formed cases*)
+  2,3: cbv in wfc; discriminate wfc.
+
+  + destruct decide.
+    {
+      apply pf_iff_split; wf_auto2.
+      toMLGoal. wf_auto2. mlIntro. mlDestructAnd "0". mlSplitAnd.
+      { mlExact "1". }
+      {
+        mlSplitAnd.
+        * mlExact "1".
+        * mlExact "2".
+      }
+      toMLGoal. wf_auto2. mlIntro. mlDestructAnd "0". mlDestructAnd "2". mlSplitAnd.
+      * mlExact "1".
+      * mlExact "3".
+    }
+    { apply pf_iff_split;[wf_auto2|wf_auto2|aapply A_impl_A|aapply A_impl_A];wf_auto2. }
+  + pose proof (IH1 := IHsz cpatt1).
+    feed specialize IH1.
+    { wf_auto2. }
+    { lia. }
+    pose proof (IH2 := IHsz cpatt2).
+    feed specialize IH2.
+    { wf_auto2. }
+    { lia. }
+
+    remember_constraint as pi.
+    assert (H : forall a b c, (Γ ⊢i a and b <---> a and c using pi) = (Γ ⊢i b <---> c using pi)).
+    {
+      intros.
+      admit.
+    }
+    clear H.
+
+    toMLGoal.
+    { wf_auto2. }
+    admit.
+  + pose proof (IH1 := IHsz cpatt1).
+    feed specialize IH1.
+    { wf_auto2. }
+    { lia. }
+    pose proof (IH2 := IHsz cpatt2).
+    feed specialize IH2.
+    { wf_auto2. }
+    { lia. }
+    admit.
+  + pose proof (IH := IHsz (ex , cpatt)).
+    feed specialize IH.
+    { wf_auto2. }
+    { simpl. admit. }
+    admit.
+  + pose proof (IH := IHsz (mu , cpatt)).
+    feed specialize IH.
+    { wf_auto2. }
+    { simpl. admit. }
+    assumption.
+Admitted.
+
+Lemma mu_and_predicate_propagation {Σ : Signature} {syntax : Syntax} i Γ ϕ ψ X :
+  well_formed (mu, ϕ) ->
+  well_formed ψ ->
+  svar_is_fresh_in X ϕ ->
+  svar_is_fresh_in X ψ ->
+  ProofInfoLe AnyReasoning i ->
+  Γ ⊢i is_predicate_pattern ψ using i ->
+  Γ ⊢i (mu, (ψ and ϕ)) <---> (ψ and (mu, ϕ)) using i.
+Proof.
+  intros wfm wfψ fϕ fψ pile Hp.
+
+  apply pf_iff_split.
+  { clear -wfm wfψ. wf_auto2. admit. }
+  { wf_auto2. }
+  
+  (* Makes set_solver work later in the proof. *)
+  unfold svar_is_fresh_in in fϕ, fψ.
+  
+  {
+    toMLGoal.
+    { wf_auto2. admit. }
+    mlIntro "H".
+    mlSplitAnd; fromMLGoal.
+    {
+      apply Knaster_tarski.
+      { eapply pile_trans;[|apply pile]. try_solve_pile. }
+      { wf_auto2. admit. }
+      unfold instantiate.
+      mlSimpl.
+      rewrite -> well_formed_bsvar_subst with (k := 0).
+      toMLGoal.
+      { wf_auto2. }
+      mlIntro.
+      mlDestructAnd "0".
+      mlExact "1".
+      { lia. }
+      { wf_auto2. }
+    }
+    {
+      rewrite <- svar_quantify_svar_open with (n := 0) (phi := (ψ and ϕ)) (X := X).
+      rewrite <- svar_quantify_svar_open with (n := 0) (phi := ϕ) (X := X) at 2.
+      apply mu_monotone.
+      { eapply pile_trans;[|apply pile]. try_solve_pile. }
+      { wf_auto2. admit. }
+      { wf_auto2. }
+      {
+        unfold svar_open.
+        mlSimpl.
+        gapply pf_conj_elim_r.
+        { eapply pile_trans;[|apply pile]. try_solve_pile. }
+        { wf_auto2. }
+        { wf_auto2. }
+      }
+      { assumption. }
+      { wf_auto2. }
+      { set_solver. }
+      { wf_auto2. }
+    }
+  }
+  
+  {
+    toMLGoal.
+    { wf_auto2. admit. }
+    mlRewrite (useBasicReasoning i (@patt_and_comm Σ Γ ψ (mu , ϕ) wfψ wfm)) at 1.
+    2: { eapply pile_trans;[|apply pile]. try_solve_pile. }
+    fromMLGoal.
+    apply lhs_from_and.
+    { wf_auto2. }
+    { wf_auto2. }
+    { wf_auto2. admit. }
+
+    apply Knaster_tarski.
+    { eapply pile_trans;[|apply pile]. try_solve_pile. }
+    { wf_auto2. }
+
+    apply lhs_to_and.
+    { wf_auto2. admit. }
+    { wf_auto2. }
+    { wf_auto2. admit. }
+    
+    toMLGoal.
+    { wf_auto2. admit. admit. }
+    assert (Htmp : is_true (well_formed (mu , ϕ) ^ [ψ ---> (mu , ψ and ϕ)])).
+    {
+      wf_auto2. admit.
+    }
+    mlRewrite (useBasicReasoning i (@patt_and_comm Σ Γ ((mu , ϕ) ^ [ψ ---> (mu , ψ and ϕ)]) ψ Htmp wfψ)) at 1.
+    2: { eapply pile_trans;[|apply pile]. try_solve_pile. }
+    
+    mlIntro "H".
+    mlApplyMeta Pre_fixp.
+    2: { wf_auto2. admit. }
+    unfold instantiate.
+    mlSimpl.
+    fromMLGoal.
+    rewrite -> well_formed_bsvar_subst with (φ := ψ) (k := 0).
+    2: auto.
+    2: wf_auto2.
+
+    remember (evar_fresh_s (free_evars ϕ)) as x.
+    pose proof (H := pred_and_ctx_and Γ
+      {|
+        pcEvar := x;
+        pcPattern := ϕ^[svar:0↦patt_free_evar x];
+      |}
+      (ψ ---> (mu , ψ and ϕ)) ψ i).
+    unfold emplace in H. simpl in H.
+    feed specialize H.
+    { wf_auto2. admit. }
+    { wf_auto2. }
+    { wf_auto2. }
+    { assumption. }
+
+    toMLGoal.
+    { wf_auto2. admit. }
+    rewrite subst_svar_evar_svar in H.
+    { apply count_evar_occurrences_0. subst. apply set_evar_fresh_is_fresh'. }
+    rewrite subst_svar_evar_svar in H.
+    { apply count_evar_occurrences_0. subst. apply set_evar_fresh_is_fresh'. }
+    clear Htmp.
+    unshelve(epose proof (Htmp := @liftPi _ _ _ _ i _ H)).
+    { eapply pile_trans;[|apply pile]. apply pile_any. }
+    mlRewrite Htmp at 1.
+    2: { eapply pile_trans;[|apply pile]. apply pile_any. }
+
+    clear Heqx x H Htmp.
+
+    remember (evar_fresh_s (free_evars ϕ)) as x.
+    pose proof (H := impl_ctx_impl_pos Γ
+      {|
+        pcEvar := x;
+        pcPattern := ϕ^[svar:0↦patt_free_evar x];
+      |}
+      (ψ and (ψ ---> (mu , ψ and ϕ)))
+      (mu , ψ and ϕ)
+      i
+      ).
+    unfold emplace in H. simpl in H.
+    feed specialize H.
+    { wf_auto2. admit. }
+    { wf_auto2. admit. }
+    { wf_auto2. }
+    { unfold is_positive_context. cbn.
+      unfold well_formed in wfm.
+      cbn in wfm.
+      destruct_and! wfm. clear -H2 Heqx.
+      apply no_neg_svar_subst.
+      { subst. eapply evar_is_fresh_in_richer'. 2: apply set_evar_fresh_is_fresh. set_solver. }
+      { assumption. }
+    }
+    { eapply pile_trans;[|apply pile]. try_solve_pile. }
+    toMLGoal.
+    { wf_auto2. admit. admit. }
+    { mlIntro "H". mlDestructAnd "H". mlApply "1". mlExact "0". }
+
+    rewrite subst_svar_evar_svar in H.
+    {
+      apply count_evar_occurrences_0. subst. apply set_evar_fresh_is_fresh'.
+    }
+    
+    rewrite subst_svar_evar_svar in H.
+    {
+      apply count_evar_occurrences_0. subst. apply set_evar_fresh_is_fresh'.
+    }
+
+    mlIntro "H".
+    mlDestructAnd "H" as "H0" "H1".
+    mlSplitAnd.
+    + mlExact "H0".
+    + mlApplyMeta H. mlExact "H1".
+  }
+Admitted. (* TODO: This lemma is awaiting for wf_auto2 to be smart enough for (mu , ϕ and ψ ) *)
+
+Theorem deduction_theorem {Σ : Signature} {syntax : Syntax} Γ ϕ ψ
+  (gpi : ProofInfo)
+  (pf : Γ ∪ {[ ψ ]} ⊢i ϕ using gpi) :
+  well_formed ϕ ->
+  well_formed ψ ->
+  theory ⊆ Γ ->
+  pi_generalized_evars gpi ## (gset_to_coGset (free_evars ψ)) ->
+  pi_substituted_svars gpi ## (gset_to_coGset (free_svars ψ)) ->
+  Γ ⊢i ⌊ ψ ⌋ ---> ϕ
+  using AnyReasoning.
+Proof.
+  intros wfϕ wfψ HΓ HnoExGen HnoSvarSubst.
+  destruct pf as [pf Hpf]. simpl.
+  induction pf.
+  - (* hypothesis *)
+    rename axiom into axiom0.
+    (* We could use [apply elem_of_union in e; destruct e], but that would be analyzing Prop
+        when building Set, which is prohibited. *)
+    destruct (decide (axiom0 = ψ)).
+    + subst.
+      eapply useGenericReasoning.
+      2: {
+        apply total_phi_impl_phi; assumption.
+      }
+      {
+        apply pile_evs_svs_kt.
+        {
+          clear. set_solver.
+        }
+        {
+          clear. set_solver.
+        }
+        { reflexivity. }
+        { clear. set_solver. }
+      }
+
+    + assert (axiom0 ∈ Γ).
+      { clear -e n. set_solver. }
+      toMLGoal.
+      { wf_auto2. }
+      mlIntro. mlClear "0". fromMLGoal.
+      eapply useGenericReasoning.
+      2: apply (hypothesis Γ axiom0 i H).
+      apply pile_evs_svs_kt.
+      {
+        set_solver.
+      }
+      {
+        set_solver.
+      }
+      {
+        simpl. reflexivity.
+      }
+      { clear. set_solver. }
+  - (* P1 *)
+    toMLGoal.
+    { wf_auto2. }
+    do 3 mlIntro. mlExactn 1.
+  - (* P2 *)
+    toMLGoal.
+    { wf_auto2. }
+    mlIntro. mlClear "0". fromMLGoal.
+    useBasicReasoning.
+    apply P2; assumption.
+  - (* P3 *)
+    toMLGoal.
+    { wf_auto2. }
+    mlIntro. mlClear "0". fromMLGoal.
+    useBasicReasoning.
+    apply P3; assumption.
+  - (* Modus Ponens *)
+    assert (well_formed phi2).
+    { unfold well_formed, well_formed_closed in *. simpl in *.
+      destruct_and!. split_and!; auto.
+    }
+    assert (well_formed phi1).
+    {
+      clear -pf1. apply proved_impl_wf in pf1. exact pf1.
+    }
+
+    remember_constraint as i'.
+
+    destruct Hpf as [Hpf2 Hpf3 Hpf4].
+    simpl in Hpf2, Hpf3, Hpf4.
+    feed specialize IHpf1.
+    {
+      constructor; simpl.
+      { set_solver. }
+      { set_solver. }
+      { unfold implb in *.
+        destruct (uses_kt pf1) eqn:Hktpf1;[|reflexivity]. simpl in *.
+        exact Hpf4.
+      }
+      { clear -pwi_pf_fp. set_solver. }
+    }
+    { assumption. }
+    feed specialize IHpf2.
+    {
+      constructor; simpl.
+      { set_solver. }
+      { set_solver. }
+      { unfold implb in *.
+        destruct (uses_kt pf2) eqn:Hktpf2;[|reflexivity].
+        rewrite orb_comm in Hpf4. simpl in *.
+        exact Hpf4.
+      }
+      {
+        clear -pwi_pf_fp. set_solver.
+      }
+    }
+    { wf_auto2. }
+    
+    (*
+    (* simplify the constraint *)
+    unfold dt_exgen_from_fp. simpl.
+    rewrite map_app.
+    rewrite list_to_set_app_L.
+    simpl.
+    *)
+
+    (*
+    (* weaken the induction hypotheses so that their constraint
+        matches the constraint of the goal *)
+    apply useGenericReasoning with (i := i') in IHpf1.
+    2: {
+      subst i'.
+      apply pile_evs_svs_kt.
+      { clear. set_solver. }
+      { clear. set_solver. }
+      { reflexivity. }
+    }
+
+    apply useGenericReasoning with (i := i') in IHpf2.
+    2: {
+      subst i'.
+      apply pile_evs_svs_kt.
+      { clear. set_solver. }
+      { clear. set_solver. }
+      { reflexivity. }
+    }
+    *)
+
+    toMLGoal.
+    { wf_auto2. }
+    mlIntro.
+    mlAdd IHpf2.
+    mlAssert ((phi1 ---> phi2)).
+    { wf_auto2. }
+    { mlApply "1". mlExactn 1. }
+    mlApply "2".
+    mlAdd IHpf1.
+    mlApply "3".
+    mlExactn 2.
+  - (* Existential Quantifier *)
+    toMLGoal.
+    { wf_auto2. }
+    mlIntro. mlClear "0". fromMLGoal.
+    useBasicReasoning.
+    apply Ex_quan. wf_auto2.
+  - (* Existential Generalization *)
+    destruct Hpf as [Hpf2 Hpf3 Hpf4].
+    simpl in Hpf2, Hpf3, Hpf4.
+    (*
+    simpl in HnoExGen.
+    case_match;[congruence|]. *)
+    feed specialize IHpf.
+    {
+      constructor; simpl.
+      { clear -Hpf2. set_solver. }
+      { clear -Hpf3. set_solver. }
+      { apply Hpf4. }
+      { clear -pwi_pf_fp. set_solver. }
+    }
+    { clear pwi_pf_fp. wf_auto2. }
+
+    apply reorder_meta in IHpf.
+    2-4: clear pwi_pf_fp; wf_auto2.
+    apply Ex_gen with (x := x) in IHpf.
+    3: { simpl. set_solver. }
+    2: { apply pile_evs_svs_kt.
+      { clear -Hpf2. set_solver. }
+      { set_solver. }
+      { reflexivity. }
+      { clear. set_solver. }
+    }
+    apply reorder_meta in IHpf.
+    2-4: clear pwi_pf_fp; wf_auto2.
+    exact IHpf.
+    
+  - (* Propagation of ⊥, left *)
+    toMLGoal.
+    { wf_auto2. }
+    mlIntro. mlClear "0". fromMLGoal.
+    useBasicReasoning.
+    apply Prop_bott_left; assumption.
+  - (* Propagation of ⊥, right *)
+    toMLGoal.
+    { wf_auto2. }
+    mlIntro. mlClear "0"; auto. fromMLGoal.
+    useBasicReasoning.
+    apply Prop_bott_right; assumption.
+  - (* Propagation of 'or', left *)
+    toMLGoal.
+    { wf_auto2. }
+    mlIntro. mlClear "0"; auto. fromMLGoal.
+    useBasicReasoning.
+    apply Prop_disj_left; assumption.
+  - (* Propagation of 'or', right *)
+    toMLGoal.
+    { wf_auto2. }
+    mlIntro. mlClear "0"; auto. fromMLGoal.
+    useBasicReasoning.
+    apply Prop_disj_right; assumption.
+  - (* Propagation of 'exists', left *)
+    toMLGoal.
+    { wf_auto2. }
+    mlIntro. mlClear "0"; auto. fromMLGoal.
+    useBasicReasoning.
+    apply Prop_ex_left; assumption.
+  - (* Propagation of 'exists', right *)
+    toMLGoal.
+    { wf_auto2. }
+    mlIntro. mlClear "0"; auto. fromMLGoal.
+    useBasicReasoning.
+    apply Prop_ex_right; assumption.
+  - (* Framing left *)
+    assert (well_formed (phi1)).
+    { unfold well_formed,well_formed_closed in *. simpl in *.
+      destruct_and!. split_and!; auto. }
+
+    assert (well_formed (phi2)).
+    { unfold well_formed,well_formed_closed in *. simpl in *.
+      destruct_and!. split_and!; auto. }
+
+    assert (well_formed (psi)).
+    { unfold well_formed,well_formed_closed in *. simpl in *.
+      destruct_and!. split_and!; auto. }
+    
+    assert (well_formed (phi1 ---> phi2)).
+    { unfold well_formed,well_formed_closed in *. simpl in *.
+      destruct_and!. split_and!; auto. }
+    destruct Hpf as [Hpf2 Hpf3 Hpf4].
+    simpl in Hpf2,Hpf3,Hpf4.
+    feed specialize IHpf.
+    {
+      constructor; simpl.
+      { set_solver. }
+      { set_solver. }
+      { apply Hpf4. }
+      { clear -pwi_pf_fp. set_solver. }
+    }
+    { wf_auto2. }
+
+    remember_constraint as i'.
+
+    (*
+    apply useGenericReasoning with (i0 := i') in IHpf.
+    2: {
+      subst i'.
+      apply pile_evs_svs_kt.
+      { clear. set_solver. }
+      { apply reflexivity. }
+      { reflexivity. }
+    }
+    *)
+    assert (S2: Γ ⊢i phi1 ---> (phi2 or ⌈ ! ψ ⌉) using i').
+    { toMLGoal.
+      { clear pwi_pf_fp; wf_auto2. }
+      mlAdd IHpf. mlIntro.
+      mlAdd (useBasicReasoning i' (A_or_notA Γ (⌈ ! ψ ⌉) ltac:(clear pwi_pf_fp; wf_auto2))).
+      mlDestructOr "0".
+      - mlRight. mlExact "3".
+      - mlLeft.
+        mlApply "4". mlExact "1".
+    }
+
+    assert (S3: Γ ⊢i (⌈ ! ψ ⌉ $ psi) ---> ⌈ ! ψ ⌉ using i').
+    {
+      replace (⌈ ! ψ ⌉ $ psi)
+        with (subst_ctx (ctx_app_l AC_patt_defined psi ltac:(assumption)) (! ψ))
+        by reflexivity.
+      subst i'.
+      gapply in_context_impl_defined; auto.
+      try_solve_pile.
+    }
+
+    assert (S4: Γ ⊢i (phi1 $ psi) ---> ((phi2 or ⌈ ! ψ ⌉) $ psi) using i').
+    { 
+      unshelve (eapply Framing_left).
+      { wf_auto2. } 2: exact S2.
+      subst i'. clear. try_solve_pile.
+    }
+
+    assert (S5: Γ ⊢i (phi1 $ psi) ---> ((phi2 $ psi) or (⌈ ! ψ ⌉ $ psi)) using i').
+    {
+      pose proof (Htmp := prf_prop_or_iff Γ (ctx_app_l box psi ltac:(assumption)) phi2 (⌈! ψ ⌉)).
+      feed specialize Htmp.
+      { clear pwi_pf_fp;wf_auto2. }
+      { clear pwi_pf_fp;wf_auto2. }
+      simpl in Htmp.
+      apply pf_iff_proj1 in Htmp.
+      3: clear pwi_pf_fp; wf_auto2.
+      2: clear pwi_pf_fp; wf_auto2.
+      subst i'.
+      eapply syllogism_meta.
+      5: {
+        gapply Htmp.
+        clear. try_solve_pile.
+      }
+      4: assumption.
+      all: clear pwi_pf_fp; wf_auto2.
+    }
+
+    assert (S6: Γ ⊢i ((phi2 $ psi) or (⌈ ! ψ ⌉ $ psi)) ---> ((phi2 $ psi) or (⌈ ! ψ ⌉)) using i').
+    {
+      toMLGoal.
+      { clear pwi_pf_fp; wf_auto2. }
+      mlIntro. mlAdd S3.
+      (* TODO we need a tactic for adding  something with stronger constraint. *)
+      mlAdd (useBasicReasoning i' (A_or_notA Γ (phi2 $ psi) ltac:(auto))).
+      mlDestructOr "2".
+      - mlLeft. mlExact "3".
+      - mlRight. mlApply "1". mlApply "0". mlExactn 0.
+    }
+
+    assert (S7: Γ ⊢i (phi1 $ psi) ---> ((phi2 $ psi)  or ⌈ ! ψ ⌉) using i').
+    {
+      toMLGoal.
+      { clear pwi_pf_fp; wf_auto2. }
+      mlAdd S5. mlAdd S6. mlIntro.
+      mlAssert (((phi2 $ psi) or (⌈ ! ψ ⌉ $ psi))).
+      { clear pwi_pf_fp; wf_auto2. }
+      { mlApply "0". mlExactn 2. }
+      mlDestructOr "3".
+      - mlLeft. mlExactn 3.
+      - mlApply "1". mlRight. mlExactn 3.
+    }
+
+    toMLGoal.
+    { clear pwi_pf_fp; wf_auto2. }
+    do 2 mlIntro. mlAdd S7.
+    mlAssert ((phi2 $ psi or ⌈ ! ψ ⌉)).
+    { clear pwi_pf_fp; wf_auto2. }
+    { mlApply "2". mlExactn 2. }
+    mlDestructOr "3".
+    + mlExactn 3.
+    + mlAssert ((phi2 $ psi or ⌈ ! ψ ⌉)).
+      { clear pwi_pf_fp; wf_auto2. }
+      { mlApply "2". mlExactn 2. }
+      mlAdd (useBasicReasoning i' (A_or_notA Γ (phi2 $ psi) ltac:(auto))).
+      mlDestructOr "4".
+      * mlExactn 0.
+      * mlAdd (useBasicReasoning i' (bot_elim Γ (phi2 $ psi) ltac:(auto))).
+        mlApply "4".
+        mlApply "0".
+        mlExactn 5.
+  - (* Framing right *)
+    assert (well_formed (phi1)).
+    { unfold well_formed,well_formed_closed in *. simpl in *.
+      destruct_and!. split_and!; auto. }
+
+    assert (well_formed (phi2)).
+    { unfold well_formed,well_formed_closed in *. simpl in *.
+      destruct_and!. split_and!; auto. }
+
+    assert (well_formed (psi)).
+    { unfold well_formed,well_formed_closed in *. simpl in *.
+      destruct_and!. split_and!; auto. }
+
+    assert (well_formed (phi1 ---> phi2)).
+    { unfold well_formed,well_formed_closed in *. simpl in *.
+      destruct_and!. split_and!; auto. }
+    simpl in HnoExGen. simpl in HnoSvarSubst.
+
+    destruct Hpf as [Hpf2 Hpf3 Hpf4].
+    simpl in Hpf2,Hpf3,Hpf4.
+    feed specialize IHpf.
+    {
+      constructor; simpl.
+      { set_solver. }
+      { set_solver. }
+      { apply Hpf4. }
+      { clear -pwi_pf_fp. set_solver. }
+    }
+    { wf_auto2. }
+
+
+    remember_constraint as i'.
+
+    (*
+    apply useGenericReasoning with (i := i') in IHpf.
+    2: {
+      subst i'.
+      apply pile_evs_svs_kt.
+      { clear. set_solver. }
+      { apply reflexivity. }
+      { reflexivity. }
+    }
+    *)
+    assert (S2: Γ ⊢i phi1 ---> (phi2 or ⌈ ! ψ ⌉) using i').
+    { toMLGoal.
+      { clear pwi_pf_fp; wf_auto2. }
+      mlAdd IHpf. mlIntro.
+      mlAdd (useBasicReasoning i' (A_or_notA Γ (⌈ ! ψ ⌉) ltac:(clear pwi_pf_fp;wf_auto2))).
+      mlDestructOr "2".
+      - mlRight. mlExactn 0.
+      - mlLeft.
+        mlAssert((phi1 ---> phi2)).
+        { wf_auto2. }
+        { mlApply "0". mlExactn 0. }
+        mlApply "2". mlExactn 2.
+    }
+
+    assert (S3: Γ ⊢i (psi $ ⌈ ! ψ ⌉) ---> ⌈ ! ψ ⌉ using i').
+    {
+      replace (psi $ ⌈ ! ψ ⌉)
+        with (subst_ctx (ctx_app_r psi AC_patt_defined ltac:(assumption)) (! ψ))
+        by reflexivity.
+        subst i'.
+        gapply in_context_impl_defined; auto.
+        try_solve_pile.
+    }
+
+    assert (S4: Γ ⊢i (psi $ phi1) ---> (psi $ (phi2 or ⌈ ! ψ ⌉)) using i').
+    { 
+      (* TODO: have a variant of apply which automatically solves all wf constraints.
+        Like: unshelve (eapply H); try_wfauto
+      *)
+      unshelve (eapply Framing_right).
+      { clear pwi_pf_fp; wf_auto2. }
+      2: exact S2.
+      subst i'. try_solve_pile.
+    }
+
+    assert (S5: Γ ⊢i (psi $ phi1) ---> ((psi $ phi2) or (psi $ ⌈ ! ψ ⌉)) using i').
+    {
+      pose proof (Htmp := prf_prop_or_iff Γ (ctx_app_r psi box ltac:(assumption)) phi2 (⌈! ψ ⌉)).
+      feed specialize Htmp.
+      { clear pwi_pf_fp; wf_auto2. }
+      { clear pwi_pf_fp; wf_auto2. }
+      simpl in Htmp.
+      apply pf_iff_proj1 in Htmp.
+      2,3: clear pwi_pf_fp; wf_auto2.
+      subst i'.
+      eapply syllogism_meta.
+      5: gapply Htmp; try_solve_pile.
+      4: assumption.
+      all: clear pwi_pf_fp; wf_auto2.
+    }
+
+    assert (S6: Γ ⊢i ((psi $ phi2) or (psi $ ⌈ ! ψ ⌉)) ---> ((psi $ phi2) or (⌈ ! ψ ⌉)) using i').
+    {
+      toMLGoal.
+      { clear pwi_pf_fp; wf_auto2. }
+      mlIntro. mlAdd S3.
+      mlAdd (useBasicReasoning i' (A_or_notA Γ (psi $ phi2) ltac:(auto))).
+      mlDestructOr "2".
+      - mlLeft. mlExactn 0.
+      - mlRight. mlApply "1". mlApply "0". mlExactn 0.
+    }
+
+    assert (S7: Γ ⊢i (psi $ phi1) ---> ((psi $ phi2)  or ⌈ ! ψ ⌉) using i').
+    {
+      toMLGoal.
+      { clear pwi_pf_fp; wf_auto2. }
+      mlAdd S5. mlAdd S6. mlIntro.
+      mlAssert (((psi $ phi2) or (psi $ ⌈ ! ψ ⌉))).
+      { clear pwi_pf_fp; wf_auto2. }
+      { mlApply "0". mlExactn 2. }
+      mlDestructOr "3".
+      - mlLeft. mlExactn 3.
+      - mlApply "1". mlRight. mlExactn 3.
+    }
+
+    toMLGoal.
+    { clear pwi_pf_fp; wf_auto2. }
+    do 2 mlIntro. mlAdd S7.
+    mlAssert ((psi $ phi2 or ⌈ ! ψ ⌉)).
+    { clear pwi_pf_fp; wf_auto2. }
+    { mlApply "2". mlExactn 2. }
+    mlDestructOr "3".
+    + mlExactn 3.
+    + mlAssert ((psi $ phi2 or ⌈ ! ψ ⌉)).
+      { clear pwi_pf_fp; wf_auto2. }
+      { mlApply "2". mlExactn 2. }
+      mlAdd (useBasicReasoning i' (A_or_notA Γ (psi $ phi2) ltac:(auto))).
+      mlDestructOr "4".
+      * mlExactn 0.
+      * mlAdd (useBasicReasoning i' (bot_elim Γ (psi $ phi2) ltac:(auto))).
+        mlApply "4".
+        mlApply "0".
+        mlExactn 5.
+  - (* Set variable substitution *)
+    simpl in HnoExGen. simpl in HnoSvarSubst. simpl in IHpf.
+    destruct Hpf as [Hpf2 Hpf3 Hpf4].
+    simpl in Hpf2, Hpf3, Hpf4.
+    feed specialize IHpf.
+    {
+      constructor; simpl.
+      { exact Hpf2. }
+      { clear -Hpf3. set_solver. }
+      { exact Hpf4. }
+      { clear -pwi_pf_fp. set_solver. }
+    }
+    {
+      clear pwi_pf_fp; wf_auto2.
+    }
+    
+    remember_constraint as i'.
+
+    replace (⌊ ψ ⌋ ---> phi^[[svar: X ↦ psi]])
+      with ((⌊ ψ ⌋ ---> phi)^[[svar: X ↦ psi]]).
+    2: {  simpl.
+        rewrite [ψ^[[svar: X ↦ psi]]]free_svar_subst_fresh.
+        {
+          clear -HnoSvarSubst Hpf3. unfold svar_is_fresh_in. set_solver.
+        }
+        reflexivity.
+    }
+    apply Svar_subst.
+    3: {
+      apply IHpf.
+    }
+    {
+      subst i'.
+      apply pile_evs_svs_kt.
+      {
+        clear. set_solver.
+      }
+      {
+        clear -Hpf3. set_solver.
+      }
+      {
+        reflexivity.
+      }
+      { clear. set_solver. }
+    }
+    { clear pwi_pf_fp; wf_auto2. }
+
+  - (* Prefixpoint *)
+    toMLGoal.
+    { wf_auto2. }
+    mlIntro. mlClear "0". fromMLGoal.
+    apply useBasicReasoning.
+    apply Pre_fixp. wf_auto2.
+  - (* Knaster-Tarski *)
+    destruct Hpf as [Hpf2 Hpf3 Hpf4].
+    apply lhs_to_and.
+    1-3: clear Hpf2 Hpf3 Hpf4 pwi_pf_fp; wf_auto2.
+    remember_constraint as pi.
+
+    epose proof (Htmp := @mu_and_predicate_propagation _ _ pi Γ phi ⌊ ψ ⌋ _ _ _ _).
+    feed specialize Htmp.
+    { apply set_svar_fresh_is_fresh. }
+    { subst pi. simpl. try_solve_pile. }
+    { eapply (liftPi _ _ _ _ (@floor_is_predicate _ _ _ _ _ _)). }
+    toMLGoal.
+    { clear Hpf2 Hpf3 Hpf4 pwi_pf_fp; wf_auto2. }
+    mlIntro.
+    apply pf_iff_proj2 in Htmp.
+    mlApplyMeta Htmp in "0". clear Htmp.
+    fromMLGoal.
+    apply Knaster_tarski.
+    { subst pi. try_solve_pile. }
+    1,3,4:clear Hpf2 Hpf3 Hpf4 pwi_pf_fp; wf_auto2.
+    1: admit.
+
+    unfold instantiate.
+    mlSimpl.
+    apply lhs_from_and.
+
+    1-3:clear Hpf2 Hpf3 Hpf4 pwi_pf_fp; wf_auto2.
+    
+    rewrite -> well_formed_bsvar_subst with (k := 0).
+    simpl in IHpf.
+    apply IHpf.
+    constructor; try assumption.
+    {
+      clear -Hpf4.
+      destruct (uses_kt pf) eqn:H; rewrite H; simpl.
+      2: reflexivity.
+      simpl in Hpf4.
+      assumption.
+    }
+    { clear -wfϕ; wf_auto2. }
+    { lia. }
+    { clear -wfψ; wf_auto2. } 
+
+
+  - (* Existence *)
+    toMLGoal.
+    { wf_auto2. }
+    mlIntro. mlClear "0". fromMLGoal.
+    apply useBasicReasoning.
+    apply Existence.
+  - (* Singleton *)
+    toMLGoal.
+    { wf_auto2. }
+    mlIntro. mlClear "0". fromMLGoal.
+    apply useBasicReasoning.
+    apply Singleton_ctx. wf_auto2.
+Admitted.
+
+Close Scope ml_scope.
+Close Scope string_scope.
+Close Scope list_scope.
